Syntax.thy
@@ -53,6 +53,9 @@ and "alt_list" =
 | ACons "alt" "alt_list"
 and "alt" =
   MatchCtor "ctor_name" tys::"tyvar list" vals::"var list" e::"term" binds tys vals in e
+lemmas term_supp = term_alt_list_alt.supp(1-8)
+lemmas alt_list_supp = term_alt_list_alt.supp(9,10)
+lemmas alt_supp = term_alt_list_alt.supp(11)
 
 nominal_datatype "binder" =
   BVar "var" "\<tau>"
@@ -87,6 +90,8 @@ lemma no_tyvars_in_kinds[simp]: "atom (a :: tyvar) \<sharp> (k :: \<kappa>)"
 
 lemma supp_empty_kinds[simp]: "supp (k :: \<kappa>) = {}"
   by (induction k rule: \<kappa>.induct) (auto simp: \<kappa>.supp)
+lemma supp_empty_kind_list[simp]: "supp (ks :: \<kappa> list) = {}"
+  by (induction ks) (auto simp: supp_Nil supp_Cons)
 
 lemma perm_data_name_var[simp]: "((a::var) \<leftrightarrow> b) \<bullet> (T :: data_name) = T"
   using flip_fresh_fresh pure_fresh by blast
